slow progress on compiler correctness
mainly trying to prove that adding/removing junk from environments is
allowed by the semantics of the intermediate language. this is
significantly complicated by closures, and relies on the intermediate
language semantics forcing canonical environments for its closures.

defined, programmatically, EVERY_Cexp and EVERY_Cv for mapping over
those types with a predicate. a little complicated because of the mutual
recursion between them.

examples/miniML/compiler/compileCorrectnessScript.sml
@@ -1,4 +1,4 @@
-open HolKernel bossLib boolLib intLib listTheory finite_mapTheory pred_setTheory lcsymtacs
+open HolKernel bossLib boolLib intLib listTheory finite_mapTheory pred_setTheory sortingTheory alistTheory SatisfySimps lcsymtacs
 open MiniMLTheory evaluateEquationsTheory compileTerminationTheory count_expTheory
 
 val _ = new_theory "compileCorrectness"
@@ -16,6 +16,7 @@ first_assum (ho_match_mp_tac o MP_CANON) >>
 rw[Abbr`ff`] >>
 TRY (Cases_on `h` >> rw[]) >>
 metis_tac[])
+val _ = export_rewrites["FINITE_free_vars"]
 
 (* TODO: move where? *)
 
@@ -173,6 +174,7 @@ val doPrim2_def = CompileTheory.doPrim2_def
 val i0_def = CompileTheory.i0_def
 val Cevaluate_ind = CompileTheory.Cevaluate_ind
 val Cevaluate_strongind = CompileTheory.Cevaluate_strongind
+val mk_env_def = CompileTheory.mk_env_def
 
 val (Cevaluate_list_with_rules,Cevaluate_list_with_ind,Cevaluate_list_with_cases) = Hol_reln [ANTIQUOTE(
 Cevaluate_rules |> SIMP_RULE (srw_ss()) [] |> concl |>
@@ -250,7 +252,7 @@ rw[Once Cevaluate_cases])
 
 val Cevaluate_fun = store_thm(
 "Cevaluate_fun",
-``∀env ns b res. Cevaluate env (CFun ns b) res = (res = Rval (CClosure (mk_env env b) ns b))``,
+``∀env ns b res. Cevaluate env (CFun ns b) res = (res = Rval (CClosure (mk_env env b (set ns)) ns b))``,
 rw[Once Cevaluate_cases])
 
 val _ = export_rewrites["Cevaluate_raise","Cevaluate_val","Cevaluate_var","Cevaluate_mat_nil","Cevaluate_let_nil","Cevaluate_fun"]
@@ -290,7 +292,7 @@ rw[Once Cevaluate_cases] >> PROVE_TAC[])
 val Cevaluate_proj = store_thm(
 "Cevaluate_proj",
 ``∀env exp n res. Cevaluate env (CProj exp n) res =
-  (∃m vs. Cevaluate env exp (Rval (CConv m vs)) ∧ (res = (Rval (EL n vs)))) ∨
+  (∃m vs. Cevaluate env exp (Rval (CConv m vs)) ∧ (n < LENGTH vs) ∧ (res = (Rval (EL n vs)))) ∨
   (∃err. Cevaluate env exp (Rerr err) ∧ (res = Rerr err))``,
 rw[Once Cevaluate_cases] >> PROVE_TAC[])
 
@@ -321,6 +323,80 @@ val Cevaluate_list_with_cons = store_thm(
   (∃v err. f e (Rval v) ∧ Cevaluate_list_with f es (Rerr err) ∧ (res = Rerr err)) ∨
   (∃err. f e (Rerr err) ∧ (res = Rerr err))``,
 rw[Once Cevaluate_list_with_cases] >> PROVE_TAC[])
+
+val evaluate_list_with_error = store_thm(
+"evaluate_list_with_error",
+``!P ls err. evaluate_list_with P ls (Rerr err) =
+             (∃n. n < LENGTH ls ∧ P (EL n ls) (Rerr err) ∧
+               !m. m < n ⇒ ∃v. P (EL m ls) (Rval v))``,
+gen_tac >> Induct >- rw[evaluate_list_with_nil] >>
+rw[EQ_IMP_THM,evaluate_list_with_cons] >- (
+  qexists_tac `SUC n` >>
+  rw[] >>
+  Cases_on `m` >> rw[] >- (
+    qexists_tac `v` >> rw[] ) >>
+  fs[] )
+>- (
+  qexists_tac `0` >>
+  rw[] ) >>
+Cases_on `n` >> fs[] >>
+disj1_tac >>
+first_assum (qspec_then `0` mp_tac) >>
+simp_tac(srw_ss())[] >>
+rw[] >> qexists_tac `v` >> rw[] >>
+qmatch_assum_rename_tac `n < LENGTH ls` [] >>
+qexists_tac `n` >> rw[] >>
+first_x_assum (qspec_then `SUC m` mp_tac) >>
+rw[])
+
+val evaluate_list_with_value = store_thm(
+"evaluate_list_with_value",
+``!P ls vs. evaluate_list_with P ls (Rval vs) = (LENGTH ls = LENGTH vs) ∧ ∀n. n < LENGTH ls ⇒ P (EL n ls) (Rval (EL n vs))``,
+gen_tac >> Induct >- rw[evaluate_list_with_nil,LENGTH_NIL_SYM] >>
+gen_tac >> Cases >> rw[evaluate_list_with_cons,EQ_IMP_THM] >- (
+  Cases_on `n` >> fs[] )
+>- (
+  first_x_assum (qspec_then `0` mp_tac) >>
+  rw[] ) >>
+first_x_assum (qspec_then `SUC n` mp_tac) >>
+rw[])
+
+val Cevaluate_list_with_error = store_thm(
+"Cevaluate_list_with_error",
+``!P ls err. Cevaluate_list_with P ls (Rerr err) =
+             (∃n. n < LENGTH ls ∧ P (EL n ls) (Rerr err) ∧
+               !m. m < n ⇒ ∃v. P (EL m ls) (Rval v))``,
+gen_tac >> Induct >- rw[Cevaluate_list_with_nil] >>
+rw[EQ_IMP_THM,Cevaluate_list_with_cons] >- (
+  qexists_tac `SUC n` >>
+  rw[] >>
+  Cases_on `m` >> rw[] >- (
+    qexists_tac `v` >> rw[] ) >>
+  fs[] )
+>- (
+  qexists_tac `0` >>
+  rw[] ) >>
+Cases_on `n` >> fs[] >>
+disj1_tac >>
+first_assum (qspec_then `0` mp_tac) >>
+simp_tac(srw_ss())[] >>
+rw[] >> qexists_tac `v` >> rw[] >>
+qmatch_assum_rename_tac `n < LENGTH ls` [] >>
+qexists_tac `n` >> rw[] >>
+first_x_assum (qspec_then `SUC m` mp_tac) >>
+rw[])
+
+val Cevaluate_list_with_value = store_thm(
+"Cevaluate_list_with_value",
+``!P ls vs. Cevaluate_list_with P ls (Rval vs) = (LENGTH ls = LENGTH vs) ∧ ∀n. n < LENGTH ls ⇒ P (EL n ls) (Rval (EL n vs))``,
+gen_tac >> Induct >- rw[Cevaluate_list_with_nil,LENGTH_NIL_SYM] >>
+gen_tac >> Cases >> rw[Cevaluate_list_with_cons,EQ_IMP_THM] >- (
+  Cases_on `n` >> fs[] )
+>- (
+  first_x_assum (qspec_then `0` mp_tac) >>
+  rw[] ) >>
+first_x_assum (qspec_then `SUC n` mp_tac) >>
+rw[])
 
 (* Invariants *)
 
@@ -402,21 +478,51 @@ rw[] >- (
   fs[good_G_def,good_cmaps_def] >>
   PROVE_TAC[] )
 >- (
-*)
-
-(*
-val exp_Cexp_thm = store_thm(
-"exp_Cexp_thm",``
-∀cm env Cenv exp Cexp. exp_Cexp cm env Cenv exp Cexp ⇒
-  ∀cenv res.
-    evaluate cenv env exp res ⇒
-    ∀cw. good_cmaps cenv cm cw ⇒
-      ∃Cres.
-        Cevaluate Cenv Cexp Cres ∧
-        (map_result (Cv_to_ov cw) Cres =
-         map_result v_to_ov res)``,
-ho_match_mp_tac exp_Cexp_ind >>
-rw[]
+  fs[EVERY2_EVERY,EVERY_MEM] >>
+  qpat_assum `LENGTH es = LENGTH ces` assume_tac >>
+  fsrw_tac[boolSimps.DNF_ss][MEM_ZIP] >>
+  first_x_assum (assume_tac o (CONV_RULE (RESORT_FORALL_CONV (fn [n,cenv,res,cw] => [cenv,cw,n,res] | _ => raise mk_HOL_ERR"""""")))) >>
+  pop_assum (qspecl_then [`cenv`,`cw`] mp_tac) >> rw[] >>
+  fs[GSYM RIGHT_EXISTS_IMP_THM,SKOLEM_THM] >>
+  fs[evaluate_con,Cevaluate_con] >>
+  Cases_on `do_con_check cenv cn (LENGTH Ces)` >> fs[] >> rw[] >- (
+    fs[evaluate_list_with_evaluate,evaluate_list_with_error,Cevaluate_list_with_Cevaluate,Cevaluate_list_with_error] >>
+    qexists_tac `f n (Rerr err)` >> rw[] >>
+    first_assum (qspecl_then [`n`,`Rerr err`] mp_tac) >>
+    Cases_on `f n (Rerr err)` >> rw[Cevaluate_list_with_error] >>
+    qexists_tac `n` >> rw[] >>
+    res_tac >>
+    first_x_assum (qspecl_then [`m`,`Rval v`] mp_tac) >>
+    `m < LENGTH Ces` by srw_tac[ARITH_ss][] >>
+    rw[] >>
+    Cases_on `f m (Rval v)` >> fs[] >>
+    metis_tac[] )
+  >- (
+    fs[evaluate_list_with_evaluate,Cevaluate_list_with_Cevaluate] >>
+    fs[evaluate_list_with_value,Cevaluate_list_with_value] >>
+    qexists_tac `Rval (CConv (cm ' cn) (GENLIST (λn. @v. (f n (Rval (EL n vs))) = Rval v) (LENGTH vs)))` >>
+    rw[] >- (
+      first_x_assum (qspec_then `n` mp_tac) >>
+      first_x_assum (qspec_then `n` mp_tac) >>
+      rw[] >>
+      first_x_assum (qspec_then `Rval (EL n vs)` mp_tac) >>
+      Cases_on `f n (Rval (EL n vs))` >> rw[] )
+    >- (
+      fs[good_cmaps_def,good_cm_cw_def] ) >>
+    rw[MAP_EQ_EVERY2,EVERY2_EVERY,EVERY_MEM,MEM_ZIP,pairTheory.FORALL_PROD] >>
+    rw[EL_GENLIST] >>
+    first_x_assum (qspec_then `n` mp_tac) >>
+    first_x_assum (qspec_then `n` mp_tac) >>
+    rw[] >>
+    first_x_assum (qspec_then `Rval (EL n vs)` mp_tac) >>
+    Cases_on `f n (Rval (EL n vs))` >> rw[] ) >>
+  qexists_tac `Rerr Rtype_error` >> rw[] >>
+  need Cevaluate to do a con check?
+  ) >>
+fs[evaluate_var] >> fs[] >> rw[] >>
+fs[good_G_def,good_cmaps_def] >>
+first_x_assum (match_mp_tac o GSYM) >>
+metis_tac[])
 *)
 
 val good_envs_def = Define`
@@ -446,14 +552,6 @@ ho_match_mp_tac exp_to_Cexp_ind >>
 rw[exp_to_Cexp_def,extend_def]
 *)
 
-(* TODO: move? *)
-local open sortingTheory in
-val QSORT_eq_if_PERM = store_thm(
-"QSORT_eq_if_PERM",
-``!R l1 l2. total R /\ transitive R /\ antisymmetric R /\ PERM l1 l2 ==> (QSORT R l1 = QSORT R l2)``,
-PROVE_TAC[QSORT_PERM,QSORT_SORTED,SORTED_PERM_EQ,PERM_TRANS,PERM_SYM])
-end
-
 local open relationTheory in
 (* TODO: move, or use set_relation stuff? *)
 val countable_has_linear_order = store_thm(
@@ -470,17 +568,6 @@ METIS_TAC[arithmeticTheory.LESS_EQUAL_ANTISYM,
           arithmeticTheory.LESS_EQ_TRANS,
           arithmeticTheory.LESS_EQ_CASES])
 end
-
-val FOLDL_UNION_BIGUNION = store_thm(
-"FOLDL_UNION_BIGUNION",
-``∀f ls s. FOLDL (λs x. s ∪ f x) s ls = s ∪ BIGUNION (IMAGE f (set ls))``,
-GEN_TAC THEN Induct THEN SRW_TAC[][UNION_ASSOC])
-
-val FOLDL_UNION_BIGUNION_paired = store_thm(
-"FOLDL_UNION_BIGUNION_paired",
-``∀f ls s. FOLDL (λs (x,y). s ∪ f x y) s ls = s ∪ BIGUNION (IMAGE (UNCURRY f) (set ls))``,
-GEN_TAC THEN Induct THEN1 SRW_TAC[][] THEN
-Cases THEN SRW_TAC[][UNION_ASSOC,GSYM pairTheory.LAMBDA_PROD])
 
 val Cevaluate_list_with_mono = store_thm(
 "Cevaluate_list_with_mono",
@@ -557,22 +644,411 @@ qmatch_assum_rename_tac `Cpmatch env p v = Cmatch env1` [] >>
 first_x_assum (qspec_then `env1` mp_tac) >> rw[] >>
 fs[SUBSET_DEF] >> metis_tac[])
 
-(* TODO: move *)
-val FMERGE_DOMSUB = store_thm(
-"FMERGE_DOMSUB",
-``∀m m1 m2 k. (FMERGE m m1 m2) \\ k = FMERGE m (m1 \\ k) (m2 \\ k)``,
-rw[fmap_domsub,FMERGE_DRESTRICT])
+val FOLDL2_FUPDATE_LIST = store_thm(
+"FOLDL2_FUPDATE_LIST",
+``!f1 f2 bs cs a. (LENGTH bs = LENGTH cs) ⇒
+  (FOLDL2 (λfm b c. fm |+ (f1 b c, f2 b c)) a bs cs =
+   a |++ ZIP (MAP2 f1 bs cs, MAP2 f2 bs cs))``,
+SRW_TAC[][FUPDATE_LIST,FOLDL2_FOLDL,MAP2_MAP,ZIP_MAP,MAP_ZIP,
+          rich_listTheory.FOLDL_MAP,rich_listTheory.LENGTH_MAP2,
+          LENGTH_ZIP,pairTheory.LAMBDA_PROD])
 
-val SUBMAP_FUNION_ABSORPTION = store_thm(
-"SUBMAP_FUNION_ABSORPTION",
-``!f g. f SUBMAP g = (FUNION f g = g)``,
-SRW_TAC[][SUBMAP_DEF,GSYM fmap_EQ_THM,EXTENSION,FUNION_DEF,EQ_IMP_THM]
-THEN PROVE_TAC[])
+val FOLDL2_FUPDATE_LIST_paired = store_thm(
+"FOLDL2_FUPDATE_LIST_paired",
+``!f1 f2 bs cs a. (LENGTH bs = LENGTH cs) ⇒
+  (FOLDL2 (λfm b (c,d). fm |+ (f1 b c d, f2 b c d)) a bs cs =
+   a |++ ZIP (MAP2 (λb. UNCURRY (f1 b)) bs cs, MAP2 (λb. UNCURRY (f2 b)) bs cs))``,
+rw[FOLDL2_FOLDL,MAP2_MAP,ZIP_MAP,MAP_ZIP,LENGTH_ZIP,
+   pairTheory.UNCURRY,pairTheory.LAMBDA_PROD,FUPDATE_LIST,
+   rich_listTheory.FOLDL_MAP])
+
+val UNCURRY_K_I_o_FST = store_thm(
+"UNCURRY_K_I_o_FST",
+``UNCURRY K = I o FST``,
+SRW_TAC[][FUN_EQ_THM,pairTheory.LAMBDA_PROD,pairTheory.FORALL_PROD])
+
+val num_Cv_linear_order_linear = store_thm(
+"a_linear_order_linear",
+``total (a_linear_order:num#Cv->num#Cv->bool) ∧
+  transitive (a_linear_order:num#Cv->num#Cv->bool) ∧
+  antisymmetric (a_linear_order:num#Cv->num#Cv->bool)``,
+fs[fsetTheory.a_linear_order_def] >>
+SELECT_ELIM_TAC >> rw[] >>
+match_mp_tac countable_has_linear_order >>
+rw[countable_def] >>
+qexists_tac `count_prod_aux count_num_aux count_Cv_aux` >>
+rw[INJ_DEF])
+
+val mk_env_canon = store_thm(
+"mk_env_canon",
+``!(env1:num|->Cv) env2 exp ns. (mk_env env1 exp ns = mk_env env2 exp ns) =
+  (∀x. x ∈ free_vars exp DIFF ns ⇒ (env1 ' x = env2 ' x))``,
+rw[mk_env_def,sort_Cenv_def] >>
+rw[num_Cv_linear_order_linear,QSORT_eq_if_PERM,PERM_fmap_to_alist,
+   fsetTheory.force_dom_def,GSYM fmap_EQ_THM] >>
+rw[FUN_FMAP_DEF])
+
+val force_dom_DRESTRICT_FUNION = store_thm(
+"force_dom_DRESTRICT_FUNION",
+``FINITE s ⇒ (force_dom fm s = (DRESTRICT fm s ⊌ (FUN_FMAP ($FAPPLY FEMPTY) s)))``,
+rw[fsetTheory.force_dom_def,GSYM fmap_EQ_THM,DRESTRICT_DEF,FUN_FMAP_DEF,FUNION_DEF] >>
+rw[EXTENSION,EQ_IMP_THM,NOT_FDOM_FAPPLY_FEMPTY])
+
+val FUN_FMAP_FAPPLY_FEMPTY_FAPPLY = store_thm(
+"FUN_FMAP_FAPPLY_FEMPTY_FAPPLY",
+``FINITE s ==> (FUN_FMAP ($FAPPLY FEMPTY) s ' x = FEMPTY ' x)``,
+Cases_on `x IN s` >>
+rw[FUN_FMAP_DEF,NOT_FDOM_FAPPLY_FEMPTY])
+val _ = export_rewrites["FUN_FMAP_FAPPLY_FEMPTY_FAPPLY"]
+
+fun PROVE_FINITE tm = prove(tm,
+  rw[pairTheory.UNCURRY] >> rw[])
+
+val FDOM_FUN_FMAP_conv = let
+  val fdomth = FUN_FMAP_DEF
+    |> SPEC_ALL
+    |> UNDISCH_ALL
+    |> CONJUNCT1
+    |> DISCH_ALL
+    |> GEN_ALL
+  val FDOM = ``FDOM``
+  val FUN_FMAP = ``FUN_FMAP``
+in
+  DEPTH_CONV (
+fn tm => let
+  val (x,fm) = dest_comb tm
+  val true = same_const x FDOM
+  val (x,[f,P]) = strip_comb fm
+  val true = same_const x FUN_FMAP
+  val th = ISPECL [f,P] fdomth
+  val (fi,_) = dest_imp (concl th)
+  val ft = PROVE_FINITE fi
+  val res = MP th ft
+in res end
+handle Bind => raise (mk_HOL_ERR""""""))
+end
+
+val FINITE_rw0 = prove(
+``FINITE (free_vars e DIFF x UNION BIGUNION (IMAGE free_vars (set ls)))``,
+rw[] >> rw[])
+val FINITE_rw1 = prove(
+``FINITE (free_vars e DIFF x UNION (free_vars e2 UNION BIGUNION (IMAGE free_vars (set ls))))``,
+rw[] >> rw[])
+val FINITE_rw2 = prove(
+``FINITE (free_vars exp DIFF setns UNION (BIGUNION (IMAGE (λ(vs,e'). free_vars e' DIFF (sset vs)) (set ls))))``,
+rw[] >> rw[pairTheory.UNCURRY])
+val FINITE_rw3 = prove(
+``FINITE (free_vars e UNION BIGUNION (IMAGE free_vars (set ls)))``,
+rw[] >> rw[])
+val _ = augment_srw_ss[rewrites[FINITE_rw0,FINITE_rw1,FINITE_rw2,FINITE_rw3]]
+
+val FUPDATE_LIST_APPLY_NOT_MEM_matchable = store_thm(
+"FUPDATE_LIST_APPLY_NOT_MEM_matchable",
+``!kvl f k v. ~MEM k (MAP FST kvl) /\ (v = f ' k) ==> ((f |++ kvl) ' k = v)``,
+PROVE_TAC[FUPDATE_LIST_APPLY_NOT_MEM])
+
+val MAP_ZIP_unfolded = let
+fun f th = let
+  val th = SPEC_ALL th
+  val tm = rand(lhs(concl th))
+  val th = PairRules.PABS tm th
+  in CONV_RULE (LAND_CONV PairRules.PETA_CONV) th end
+in
+MAP_ZIP
+|> SIMP_RULE (srw_ss()) [f pairTheory.FST,f pairTheory.SND]
+end
+
+fun mk_EVERY ty = let
+  val (name,_) = dest_type ty
+  val EVERY_ty = "EVERY_"^name
+  val P = mk_var("P"^name,ty-->bool)
+  val EVERY_ty = mk_var(EVERY_ty,(ty-->bool)-->ty-->bool)
+  val args = map (rhs o #2 o strip_exists) (strip_disj(#2(strip_forall(concl(TypeBase.nchotomy_of ty)))))
+  fun f (x,(vs,acc)) = let val v = with_flag (Globals.priming,SOME"") (variant vs) x in (v::vs,v::acc) end
+  fun g (tm,(vs,acc)) = let
+    val (c,bs) = strip_comb tm
+    val (vs,bs) = foldl f (vs,[]) bs
+  in (vs,(list_mk_comb(c,rev bs))::acc) end
+  val (_,args) = foldl g ([EVERY_ty,P],[]) args
+  fun f (tm,acc) = let val ty' = type_of tm in
+  let val ty'' = listSyntax.dest_list_type ty' in
+  let val (tya,tyb) = pairSyntax.dest_prod ty'' in
+  let
+    fun f p = listSyntax.mk_every(mk_comb(EVERY_ty,P),listSyntax.mk_map(inst[alpha|->tya,beta|->tyb]p,tm))
+    val acc = if tya = ty then (f pairSyntax.fst_tm)::acc else acc
+    val acc = if tyb = ty then (f pairSyntax.snd_tm)::acc else acc
+  in acc end
+  end handle HOL_ERR {origin_function="dest_prod",...} =>
+    if ty'' = ty then listSyntax.mk_every(mk_comb(EVERY_ty,P),tm)::acc else acc
+  end handle HOL_ERR {origin_function="dest_list_type",...} =>
+    if ty' = ty then list_mk_comb(EVERY_ty,[P,tm])::acc else acc
+  end
+  fun eq tm = mk_eq(list_mk_comb(EVERY_ty,[P,tm]),list_mk_conj((mk_comb(P,tm))::(foldl f [] (#2(strip_comb tm)))))
+  val eqs = map eq args
+in [ANTIQUOTE (list_mk_conj eqs)] end
+
+val tys = [``:Cexp``,``:Cv``]
+
+val variant_args = let
+  fun f (x,(vs,acc)) = let val v = with_flag (Globals.priming,SOME"") (variant vs) x in (v::vs,v::acc) end
+  fun g (tm,(vs,acc)) = let
+    val (c,bs) = strip_comb tm
+    val (vs,bs) = foldl f (vs,[]) bs
+  in (vs,(list_mk_comb(c,rev bs))::acc) end
+in g end
+
+fun args_from_nchotomy ty = map (rhs o #2 o strip_exists) (strip_disj(#2(strip_forall(concl(TypeBase.nchotomy_of ty)))))
+
+fun uneta tm = let
+  val (t,_) = dom_rng (type_of tm)
+  val x = genvar t
+in mk_abs(x,mk_comb(tm,x)) end
+
+fun find_tys listfn add (tm,acc) =
+let val ty' = type_of tm in
+let val ty'' = listSyntax.dest_list_type ty' in
+let val (tya,tyb) = pairSyntax.dest_prod ty'' in
+let
+  fun f p EVP = listfn(uneta EVP,listSyntax.mk_map(inst[alpha|->tya,beta|->tyb]p,tm))
+  val acc = add (f pairSyntax.fst_tm) tya acc
+  val acc = add (f pairSyntax.snd_tm) tyb acc
+in acc end
+end handle HOL_ERR {origin_function="dest_prod",...} =>
+  add (fn EVP => listfn(uneta EVP,tm)) ty'' acc
+end handle HOL_ERR {origin_function="dest_list_type",...} =>
+  add (fn EVP => mk_comb(EVP,tm)) ty' acc
+end
+
+fun lmk_conj ls = list_mk_conj ls handle HOL_ERR _ => T
+fun lmk_disj ls = list_mk_disj ls handle HOL_ERR _ => F
+
+fun mk_cvtr conjfn listfn name ty1 ty2 = let
+  val P = mk_var("P",ty1-->bool)
+  val cvtr = mk_var(name,(ty1-->bool)-->ty2-->bool)
+  val cP = mk_comb(cvtr,P)
+  val args = args_from_nchotomy ty2
+  val (_,args) = foldl variant_args ([cvtr,P],[]) args
+  fun add f ty acc = if ty = ty1 then f P :: acc else acc
+  fun eq tm = mk_eq(mk_comb(cP,tm),conjfn(foldl (find_tys listfn add) [] (#2(strip_comb tm))))
+  val eqs = map eq args
+  val eqs = list_mk_conj eqs
+in [ANTIQUOTE eqs] end
+
+val mk_every_cvtr = mk_cvtr lmk_conj listSyntax.mk_every
+val mk_exists_cvtr = mk_cvtr lmk_disj listSyntax.mk_exists
+
+fun mk_EVERY cvtr tys = let
+  val names = map (#1 o dest_type) tys
+  val EVERY_tys = map (fn n => "EVERY_"^n) names
+  val Ps = map (fn (n,ty) => mk_var("P"^n,ty-->bool)) (zip names tys)
+  val EVERY_tys = map (fn (EVERY_ty,ty) => mk_var(EVERY_ty,(ty-->bool)-->ty-->bool)) (zip EVERY_tys tys)
+  val argss = map args_from_nchotomy tys
+  fun h (tms,(vs,acc)) = let
+    val (vs,tms) = foldl variant_args (vs,[]) tms
+  in (vs,tms::acc) end
+  val (_,argss) = foldl h (EVERY_tys@Ps,[]) argss
+  fun add j f ty acc =
+    case total (index (equal ty)) tys of
+      NONE => acc
+    | SOME i => let
+      val EV = List.nth(EVERY_tys,j)
+      val P = List.nth(Ps,j)
+      val EVP = mk_comb(EV,P)
+      val EVP = if i = j then EVP else mk_comb(cvtr j i,EVP)
+      in f EVP :: acc end
+  fun eq tm = let
+    val ty = type_of tm
+    val i = index (equal ty) tys
+    val EVERY_ty = List.nth(EVERY_tys,i)
+    val P = List.nth(Ps,i)
+  in
+    mk_eq(list_mk_comb(EVERY_ty,[P,tm]),list_mk_conj((mk_comb(P,tm))::(foldl (find_tys listSyntax.mk_every (add i)) [] (#2(strip_comb tm)))))
+  end
+  val eqs = map (fn args => list_mk_conj (map eq args)) argss
+in map ANTIQUOTE eqs end
+
+val EVERY_Cbody_def = Define (mk_every_cvtr "EVERY_Cbody" ``:Cexp`` ``:Cv``)
+val EVERY_CVal_def = Define (mk_every_cvtr "EVERY_CVal" ``:Cv`` ``:Cexp``)
+val EXISTS_Cbody_def = Define (mk_exists_cvtr "EXISTS_Cbody" ``:Cexp`` ``:Cv``)
+val EXISTS_CVal_def = Define (mk_exists_cvtr "EXISTS_CVal" ``:Cv`` ``:Cexp``)
+val _ = export_rewrites["EVERY_Cbody_def","EVERY_CVal_def","EXISTS_Cbody_def","EXISTS_CVal_def"]
+
+fun cvtr 0 1 = ``EVERY_Cbody`` | cvtr 1 0 = ``EVERY_CVal``
+
+val EVERY_Cbody_cong = store_thm(
+"EVERY_Cbody_cong",
+``!P P' Cv Cv'. (Cv = Cv') ∧ (∀x. EXISTS_Cbody ($= x) Cv' ==> (P x = P' x))
+==> (EVERY_Cbody P Cv = EVERY_Cbody P' Cv')``,
+ntac 2 gen_tac >>
+Induct >> rw[] >> rw[] >> fs[] >>
+fs[EVERY_MAP,EXISTS_MAP] >>
+fs[EVERY_MEM,EXISTS_MEM] >>
+metis_tac[])
+val _ = DefnBase.export_cong"EVERY_Cbody_cong"
+
+val EVERY_CVal_cong = store_thm(
+"EVERY_CVal_cong",
+``!P P' Cv Cv'. (Cv = Cv') ∧ (∀x. EXISTS_CVal ($= x) Cv' ==> (P x = P' x))
+==> (EVERY_CVal P Cv = EVERY_CVal P' Cv')``,
+ntac 2 gen_tac >>
+Induct >> rw[] >> rw[] >> fs[] >>
+fs[EVERY_MAP,EXISTS_MAP] >>
+fs[EVERY_MEM,EXISTS_MEM] >>
+metis_tac[])
+val _ = DefnBase.export_cong"EVERY_CVal_cong"
+
+val [EVERY_Cv_eqs,EVERY_Cexp_eqs] = mk_EVERY cvtr [``:Cexp``,``:Cv``]
+
+val Cexp_size_def = CompileTheory.Cexp_size_def
+
+val EVERY_Cv_def = tDefine "EVERY_Cv" [EVERY_Cv_eqs](
+WF_REL_TAC `measure (Cv_size o SND)` >>
+srw_tac[ARITH_ss][Cexp3_size_thm,Cexp8_size_thm] >>
+Q.ISPEC_THEN `Cv_size` imp_res_tac SUM_MAP_MEM_bound >>
+fsrw_tac[ARITH_ss][SUM_MAP_Cexp5_size_thm] >>
+qmatch_assum_rename_tac `EXISTS_CVal X cv` ["X"] >>
+Cases_on`cv`>>fs[]>>rw[]>>
+fsrw_tac[ARITH_ss][Cexp_size_def,Cexp1_size_thm,SUM_MAP_Cexp2_size_thm] >>
+Q.ISPEC_THEN `Cexp_size` imp_res_tac SUM_MAP_MEM_bound >>
+fsrw_tac[ARITH_ss][Cexp_size_def])
+
+val EVERY_Cexp_def = tDefine "EVERY_Cexp" [EVERY_Cexp_eqs](
+WF_REL_TAC `measure (Cexp_size o SND)` >>
+srw_tac[ARITH_ss][Cexp7_size_thm,Cexp4_size_thm,Cexp1_size_thm] >>
+Q.ISPEC_THEN `Cexp_size` imp_res_tac SUM_MAP_MEM_bound >>
+fsrw_tac[ARITH_ss][Cexp_size_def,SUM_MAP_Cexp2_size_thm,SUM_MAP_Cexp6_size_thm] >>
+qmatch_assum_rename_tac `EXISTS_Cbody X ll` ["X"] >>
+Cases_on`ll`>>fs[]>>rw[Cexp_size_def,Cexp3_size_thm,Cexp1_size_thm,SUM_MAP_Cexp2_size_thm,SUM_MAP_Cexp5_size_thm] >>
+fs[EXISTS_MEM] >>
+Q.ISPEC_THEN `Cexp_size` imp_res_tac SUM_MAP_MEM_bound >>
+fsrw_tac[ARITH_ss][Cexp_size_def])
+
+val _ = export_rewrites["EVERY_Cv_def","EVERY_Cexp_def"]
+
+val canonical_env_def = Define`
+  (canonical_env (CClosure env ns b) = (FDOM (alist_to_fmap env) = free_vars b DIFF (set ns))) ∧
+  (canonical_env (CRecClos env ns bs n) = case find_index n ns 0 of
+    SOME i => (FDOM (alist_to_fmap env) = free_vars (SND (EL i bs)) DIFF (set (FST (EL i bs))) DIFF (set ns))
+    | NONE => F) ∧
+  (canonical_env _ = T)`
+
+val _ = export_rewrites["canonical_env_def"]
+
+val FOLDL2_Cmatch_bind_error = store_thm(
+"FOLDL2_Cmatch_bind_error",
+``∀f ps vs.
+(FOLDL2 (λa p v. Cmatch_bind a (f a p v)) Cno_match ps vs = Cno_match) ∧
+  (FOLDL2 (λa p v. Cmatch_bind a (f a p v)) Cmatch_error ps vs = Cmatch_error)``,
+gen_tac >> Induct >- (Cases >> rw[]) >>
+gen_tac >> Cases >> rw[])
+
+val Cpmatch_canonical_envs = store_thm(
+"Cpmatch_canonical_envs",
+``(∀env p v env'. (Cpmatch env p v = Cmatch env') ∧ (∀v. v ∈ FRANGE env ⇒ EVERY_Cv canonical_env v) ∧ EVERY_Cv canonical_env v ⇒ (∀v. v ∈ FRANGE env' ⇒ EVERY_Cv canonical_env v)) ∧
+(∀env ps vs env'. (Cpmatch_list env ps vs = Cmatch env') ∧ (∀v. v ∈ FRANGE env ⇒ EVERY_Cv canonical_env v) ∧ EVERY (EVERY_Cv canonical_env) vs ⇒ (∀v. v ∈ FRANGE env' ⇒ EVERY_Cv canonical_env v))``,
+ho_match_mp_tac Cpmatch_ind >>
+rw[Cpmatch_def] >>
+fs[FRANGE_DEF] >> rw[DOMSUB_FAPPLY_THM] >>
+(ASSUM_LIST (fn ls => if length ls < 7 then NO_TAC else ALL_TAC)
+ ORELSE metis_tac[]) >>
+Cases_on `Cpmatch env p v` >> fs[] >>
+qmatch_assum_rename_tac `Cpmatch env p v = Cmatch env''` [] >>
+first_x_assum (qspecl_then [`env''`,`env'`] (match_mp_tac o MP_CANON)) >>
+rw[] >>
+metis_tac[])
+
+val FST_triple = store_thm(
+"FST_triple",
+``(λ(n,ns,b). n) = FST``,
+rw[FUN_EQ_THM,pairTheory.UNCURRY])
+
+val SND_triple = store_thm(
+"SND_triple",
+``(λ(n,ns,b). f ns b) = UNCURRY f o SND``,
+rw[FUN_EQ_THM,pairTheory.UNCURRY])
+
+val MEM_QSORT = store_thm(
+"MEM_QSORT",
+``MEM x (QSORT R ls) = MEM x ls``,
+METIS_TAC[QSORT_PERM,MEM_PERM])
+val _ = export_rewrites["MEM_QSORT"]
+
+val MEM_sort_Cenv = store_thm(
+"MEM_sort_Cenv",
+``MEM x (sort_Cenv env) = MEM x env``,
+rw[sort_Cenv_def])
+val _ = export_rewrites["MEM_sort_Cenv"]
+
+val EVERY_Cexp_EVERY_CVal_imp = store_thm(
+"EVERY_Cexp_EVERY_CVal_imp",
+``∀P e. EVERY_Cexp (EVERY_CVal P) e ⇒ EVERY_CVal P e``,
+gen_tac >> Cases >> rw[])
 
 (*
+val Cevaluate_canonical_envs = store_thm(
+"Cevaluate_canonical_envs",
+``∀env exp res. Cevaluate env exp res ⇒
+  ((∀v. v ∈ FRANGE env ⇒ EVERY_Cv canonical_env v) ∧
+   (EVERY_Cexp (EVERY_CVal (EVERY_Cv canonical_env)) exp))
+⇒ ∀v. (res = Rval v) ⇒ EVERY_Cv canonical_env v``,
+ho_match_mp_tac Cevaluate_nice_ind >> rw[] >>
+TRY (
+  first_x_assum match_mp_tac >>
+  rw[FRANGE_DEF] >> metis_tac[] ) >>
+TRY (
+  fs[Cevaluate_list_with_value,EVERY_MEM,MEM_EL] >> rw[] >>
+  first_assum (qspec_then `n` (match_mp_tac o MP_CANON)) >> rw[] >>
+  first_x_assum match_mp_tac >> metis_tac[] ) >>
+TRY (
+  fs[EVERY_MEM,MEM_EL] >>
+  metis_tac[] ) >>
+TRY (
+  pop_assum mp_tac >> rw[] >>
+  `EVERY_Cv canonical_env (env ' n)` by (
+    fs[FRANGE_DEF] >> metis_tac[] ) >>
+  `∀v. v ∈ FRANGE env' ⇒ EVERY_Cv canonical_env v` by
+    imp_res_tac Cpmatch_canonical_envs >>
+  fs[] ) >>
+TRY (
+  pop_assum match_mp_tac >>
+  rw[] >> fs[] >>
+  first_x_assum match_mp_tac >>
+  fs[FRANGE_DEF] >> rw[DOMSUB_FAPPLY_THM] >>
+  metis_tac[])
+TRY (
+  pop_assum match_mp_tac >>
+  fs[FOLDL2_FUPDATE_LIST_paired] >>
+  fs[FRANGE_DEF,FDOM_FUPDATE_LIST,MAP_ZIP,MAP2_MAP,FST_triple,LENGTH_ZIP,SND_triple] >>
+  fsrw_tac[boolSimps.DNF_ss][] >>
+  fs[GSYM FORALL_AND_THM] >>
+  qx_gen_tac `x` >>
+  Cases_on `MEM x ns` >- (
+    fs[] >> conj_asm2_tac >> fs[] >>
+    fs[MEM_EL] >> rw[] >>
+    qmatch_abbrev_tac `P ((env |++ ls) ' (EL n ns))` >>
+    qsuff_tac `(env |++ ls) ' (EL n ns) = EL n (MAP SND ls)` >- (
+      qpat_assum `LENGTH ns = LENGTH defs` assume_tac >> fs[] >>
+      rw[EL_MAP,Abbr`ls`,Abbr`P`,MAP_ZIP,LENGTH_ZIP,EL_ZIP] >>
+      rw[pairTheory.UNCURRY] >- (
+        rw[EXTENSION,MEM_MAP,mk_env_def,pairTheory.EXISTS_PROD,FLOOKUP_DEF] )
+      >- (
+        fsrw_tac[boolSimps.ETA_ss][EVERY_MAP,EVERY_MEM,MEM_EL] >>
+        metis_tac[EVERY_Cexp_EVERY_CVal_imp] ) >>
+      fsrw_tac[boolSimps.ETA_ss][EVERY_MAP,mk_env_def,EVERY_MEM,pairTheory.FORALL_PROD,FLOOKUP_DEF,force_dom_DRESTRICT_FUNION,FUNION_DEF,DRESTRICT_DEF] >>
+      rw[] >> fs[]
+      )
+      rw[EL_MAP]
+
+      rw[Abbr`P`] >> metis_tac[] ) >>
+    match_mp_tac FUPDATE_LIST_APPLY_NOT_MEM >>
+    unabbrev_all_tac >>
+    rw[MAP_ZIP,LENGTH_ZIP]
+    fs[FUPDATE_LIST_APPLY_NOT_MEM,MAP_ZIP,LENGTH_ZIP]
+
 val Cevaluate_any_env = store_thm(
 "Cevaluate_any_env",
-``∀env exp res. Cevaluate env exp res ⇒ ∀env'. Cevaluate ((DRESTRICT env (free_vars exp)) ⊌ env') exp res``,
+``∀env exp res. Cevaluate env exp res ⇒ ∀env'. Cevaluate ((force_dom env (free_vars exp)) ⊌ env') exp res``,
+fs[force_dom_DRESTRICT_FUNION] >>
 ho_match_mp_tac Cevaluate_nice_ind >>
 rw[FOLDL_UNION_BIGUNION,FOLDL_UNION_BIGUNION_paired,
    FAPPLY_FUPDATE_THM,DRESTRICT_DEF,FUNION_DEF,
@@ -586,8 +1062,8 @@ TRY (
   qmatch_abbrev_tac `Cevaluate env1 e r` >>
   qsuff_tac `env0 ⊌ env1 = env1` >- PROVE_TAC[] >>
   rw[GSYM SUBMAP_FUNION_ABSORPTION] >>
-  rw[Abbr`env0`,Abbr`env1`,SUBMAP_DEF,DRESTRICT_DEF,FUNION_DEF] >>
-  srw_tac[boolSimps.DNF_ss][] >>
+  rw[Abbr`env0`,Abbr`env1`,SUBMAP_DEF,DRESTRICT_DEF,FUNION_DEF,FUN_FMAP_DEF] >>
+  srw_tac[boolSimps.DNF_ss][FUN_FMAP_DEF] >>
   metis_tac[] ) >>
 TRY (
   fs[Once Cpmatch_FEMPTY] >>
@@ -598,8 +1074,9 @@ TRY (
   qmatch_abbrev_tac `Cevaluate env1 exp res` >>
   qsuff_tac `env0 ⊌ env1 = env1` >- PROVE_TAC[] >>
   rw[GSYM SUBMAP_FUNION_ABSORPTION] >>
-  rw[Abbr`env0`,Abbr`env1`,SUBMAP_DEF,DRESTRICT_DEF,FUNION_DEF] >>
-  srw_tac[boolSimps.DNF_ss][] >>
+  rw[Abbr`env0`,Abbr`env1`,SUBMAP_DEF,DRESTRICT_DEF,FUNION_DEF,FUN_FMAP_DEF,pairTheory.UNCURRY] >>
+  srw_tac[boolSimps.DNF_ss][FUN_FMAP_DEF,pairTheory.UNCURRY] >>
+  fsrw_tac[boolSimps.DNF_ss][FUN_FMAP_DEF,pairTheory.UNCURRY] >>
   metis_tac[] ) >>
 TRY (
   disj1_tac >>
@@ -610,8 +1087,8 @@ TRY (
   qsuff_tac `(env0 ⊌ env1 = env1) ∧ (env2 ⊌ env1 |+ (n,v) = env1 |+ (n,v))` >- PROVE_TAC[] >>
   rw[GSYM SUBMAP_FUNION_ABSORPTION] >>
   rw[Abbr`env0`,Abbr`env1`,Abbr`env2`,SUBMAP_DEF,DRESTRICT_DEF,FUNION_DEF,
-     DRESTRICT_FUPDATE,FAPPLY_FUPDATE_THM] >>
-  srw_tac[boolSimps.DNF_ss][] >>
+     DRESTRICT_FUPDATE,FAPPLY_FUPDATE_THM,FUN_FMAP_DEF] >>
+  srw_tac[boolSimps.DNF_ss][FUN_FMAP_DEF] >>
   metis_tac[] ) >>
 TRY (
   disj2_tac >>
@@ -623,9 +1100,121 @@ TRY (
      DRESTRICT_FUPDATE,FAPPLY_FUPDATE_THM] >>
   srw_tac[boolSimps.DNF_ss][] >>
   metis_tac[] ) >>
+TRY (
+  rw[Once Cevaluate_cases] >>
+  qmatch_assum_abbrev_tac `∀env'. Cevaluate (env0 ⊌ env') exp res` >>
+  qmatch_abbrev_tac `Cevaluate env1 exp res` >>
+  qsuff_tac `(env0 ⊌ env1 = env1)` >- PROVE_TAC[] >>
+  rw[GSYM SUBMAP_FUNION_ABSORPTION] >>
+  qunabbrev_tac `env0` >>
+  qho_match_abbrev_tac `DRESTRICT (FOLDL2 (λenv' n (ns,b). env' |+ (n, f n ns b)) env ns defs) (free_vars exp) ⊌ femp SUBMAP env1` >>
+  Q.ISPECL_THEN [`K:num->num list#Cexp->num`,`λn:num (ns,b). f n ns b`,`ns`,`defs`,`env`] mp_tac FOLDL2_FUPDATE_LIST >>
+  rw[pairTheory.LAMBDA_PROD] >>
+  pop_assum kall_tac >> qunabbrev_tac `f` >>
+  qunabbrev_tac `env1` >>
+  qho_match_abbrev_tac `lhs SUBMAP FOLDL2 (λenv' n (ns,b). env' |+ (n, f n ns b)) a ns defs` >>
+  Q.ISPECL_THEN [`K:num->num list#Cexp->num`,`λn:num (ns,b). f n ns b`,`ns`,`defs`,`a`] mp_tac FOLDL2_FUPDATE_LIST >>
+  rw[pairTheory.LAMBDA_PROD] >>
+  pop_assum kall_tac >> unabbrev_all_tac >>
+  qpat_assum `LENGTH ns = LENGTH defs` assume_tac >>
+  fs[SUBMAP_DEF] >>
+  qx_gen_tac `x` >>
+  disch_then assume_tac >>
+  conj_tac >- (
+    fsrw_tac[boolSimps.DNF_ss][DRESTRICT_DEF,FDOM_FUPDATE_LIST,MEM_MAP,MEM_ZIP,
+                               MAP2_ZIP,MAP_ZIP,LENGTH_ZIP,pairTheory.EXISTS_PROD] >>
+    metis_tac[MEM_EL,pairTheory.pair_CASES] ) >>
+  pop_assum mp_tac >>
+  fs[DRESTRICT_DEF,FDOM_FUPDATE_LIST] >>
+  qmatch_abbrev_tac `((A \/ B) /\ C) \/ C ==> D` >>
+  qsuff_tac `C ==> D` >- (
+    rpt (pop_assum kall_tac) >> metis_tac[]) >>
+  unabbrev_all_tac >>
+  strip_tac >>
+  Cases_on `MEM x ns` >- (
+    rw[FUNION_DEF,DRESTRICT_DEF,FDOM_FUPDATE_LIST,MAP_ZIP,MEM_MAP,MEM_ZIP,MAP2_MAP, UNCURRY_K_I_o_FST,LENGTH_ZIP] >>
+    match_mp_tac FUPDATE_LIST_APPLY_MEM >>
+    fs[MAP_ZIP,LENGTH_ZIP,MEM_EL] >>
+    qpat_assum `n < LENGTH ns` mp_tac >> rw[] >>
+    qexists_tac `n` >>
+    fs[EL_MAP,LENGTH_ZIP,EL_ZIP] >>
+    conj_asm2_tac >- (
+      match_mp_tac FUPDATE_LIST_APPLY_MEM >>
+      fs[LENGTH_ZIP,MAP_ZIP] >>
+      qexists_tac `n` >>
+      fs[EL_MAP,LENGTH_ZIP,EL_ZIP] >>
+      rw[pairTheory.UNCURRY] >>
+      rw[mk_env_canon] >>
+      qmatch_abbrev_tac `env ' x = (DRESTRICT env s ⊌ f0 ⊌ f2) ' x` >>
+      qsuff_tac `x ∈ s` >- (
+        strip_tac >>
+        Cases_on `x ∈ FDOM env` >>
+        rw[FUNION_DEF,DRESTRICT_DEF,Abbr`s`,NOT_FDOM_FAPPLY_FEMPTY] ) >>
+      unabbrev_all_tac >> rw[] >>
+      disj2_tac >>
+      rw[pairTheory.UNCURRY] >>
+      metis_tac[MEM_EL,IN_DIFF,IN_LIST_TO_SET,IN_UNION] ) >>
+    fs[EL_ALL_DISTINCT_EL_EQ] ) >>
+  rw[FUNION_DEF,DRESTRICT_DEF,FDOM_FUPDATE_LIST,MAP_ZIP,MEM_MAP,MEM_ZIP,MAP2_MAP, UNCURRY_K_I_o_FST,LENGTH_ZIP] >- (
+     match_mp_tac FUPDATE_LIST_APPLY_NOT_MEM_matchable >>
+     rw[MAP_ZIP,LENGTH_ZIP] >>
+     match_mp_tac FUPDATE_LIST_APPLY_NOT_MEM_matchable >>
+     rw[MAP_ZIP,LENGTH_ZIP] >>
+     qmatch_abbrev_tac `env ' x = (DRESTRICT env s ⊌ f0 ⊌ f2) ' x` >>
+     qsuff_tac `x ∈ s` >- rw[DRESTRICT_DEF,FUNION_DEF] >>
+     rw[Abbr`s`] ) >>
+   match_mp_tac EQ_SYM >>
+   match_mp_tac FUPDATE_LIST_APPLY_NOT_MEM_matchable >>
+   rw[MAP_ZIP,LENGTH_ZIP] >>
+   qmatch_abbrev_tac `FEMPTY ' x = (DRESTRICT env s ⊌ f0 ⊌ f2) ' x` >>
+   rw[DRESTRICT_DEF,FUNION_DEF,FUN_FMAP_DEF,Abbr`s`] ) >>
+TRY (
+  rw[mk_env_canon] >>
+  qmatch_abbrev_tac `env ' x = (DRESTRICT env s ⊌ f0 ⊌ f2) ' x` >>
+  qsuff_tac `x ∈ s` >- (
+    strip_tac >>
+    Cases_on `x ∈ FDOM env` >>
+    rw[FUNION_DEF,DRESTRICT_DEF,Abbr`s`,NOT_FDOM_FAPPLY_FEMPTY] ) >>
+  rw[Abbr`s`] ) >>
+TRY (
+  rw[Once Cevaluate_cases] >>
+  disj1_tac >>
+  qmatch_assum_abbrev_tac `∀env''. Cevaluate (env0 ⊌ env'') exp (Rval (CClosure env' ns exp'))` >>
+  map_every qexists_tac [`env'`,`ns`,`exp'`,`vs`] >>
+  rw[Cevaluate_list_with_Cevaluate] >>
+  fs[Cevaluate_list_with_value] >>
+  TRY (
+    qx_gen_tac `n` >> rw[] >>
+    first_x_assum (qspec_then `n` mp_tac) >> rw[] ) >>
+  unabbrev_all_tac >>
+  qmatch_abbrev_tac `Cevaluate env1 exp1 res1` >>
+  qmatch_assum_abbrev_tac `∀env''. Cevaluate (env0 ⊌ env'') exp1 res1` >>
+  TRY (
+    rw[MAP2_MAP,MAP_ZIP_unfolded,FDOM_FUPDATE_LIST,MEM_MAP,MEM_ZIP] >>
+  )
+  qsuff_tac `env0 ⊌ env1 = env1` >- metis_tac[] >>
+  rw[GSYM SUBMAP_FUNION_ABSORPTION] >>
+  rw[SUBMAP_DEF,Abbr`env0`,Abbr`env1`,DRESTRICT_DEF,FUN_FMAP_DEF,FUNION_DEF] >>
+  srw_tac[boolSimps.DNF_ss][FUN_FMAP_DEF,MEM_EL,FOLDL2_FUPDATE_LIST] >>
+  metis_tac[]
+  >- (
+    rw[Cevaluate_list_with_Cevaluate] >>
+    fs[Cevaluate_list_with_value] >>
+    qx_gen_tac `n` >> rw[] >>
+    first_x_assum (qspec_then `n` mp_tac) >> rw[] >>
+    unabbrev_all_tac >>
+    qmatch_assum_abbrev_tac `∀env'. Cevaluate (env0 ⊌ env') (EL n es) (Rval (EL n vs))` >>
+    qmatch_abbrev_tac `Cevaluate env1 (EL n es) (Rval (EL n vs))` >>
+    qsuff_tac `env0 ⊌ env1 = env1` >- metis_tac[] >>
+    rw[GSYM SUBMAP_FUNION_ABSORPTION] >>
+    rw[SUBMAP_DEF,Abbr`env0`,Abbr`env1`,DRESTRICT_DEF,FUN_FMAP_DEF,FUNION_DEF]
+    srw_tac[boolSimps.DNF_ss][FUN_FMAP_DEF,MEM_EL] >>
+    metis_tac[] ) >>
 
 >> PROVE_TAC[]
+*)
 
+(*
 val Cevaluate_free_vars_env = save_thm(
 "Cevaluate_free_vars_env",
 Cevaluate_any_env
